More

qdt/Qdt/MLTT/Substitution/Basic.lean
@@ -1,147 +1,508 @@
-import Qdt.MLTT.Shift
+import Qdt.MLTT.Syntax
 
 namespace Qdt
 
+private def Ren (a b : Nat) := Idx a → Idx b
+private def Ren.id (a : Nat) : Ren a a := fun i => i
+private def Ren.shift {a} : Ren a (a + 1) := Fin.succ
+private def Ren.comp {l m n : Nat} (ξ : Ren l m) (ζ : Ren m n) : Ren l n := ζ ∘ ξ
+private theorem Ren.id_comp {m n} (ξ : Ren m n) : Ren.comp (Ren.id m) ξ = ξ := Function.id_comp ξ
+private theorem Ren.comp_id {m n}(ξ : Ren m n) : Ren.comp ξ (Ren.id n) = ξ := Function.comp_id ξ
+private theorem Ren.comp_assoc {k l m n} (ξ : Ren k l) (ζ : Ren l m) (η : Ren m n) :
+    (ξ.comp ζ).comp η = ξ.comp (ζ.comp η) := rfl
+
+private def Ren.cons {a b} (j : Idx b) (ξ : Ren a b) : Ren (a + 1) b
+  | ⟨0, _⟩ => j
+  | ⟨i + 1, h⟩ => ξ ⟨i, by omega⟩
+infixr:67 " .: " => Ren.cons
+
+private def Ren.up {a b} (ξ : Ren a b) : Ren (a + 1) (b + 1) := 0 .: Ren.shift ∘ ξ
+
 mutual
-
-def Ty.substAt {n} (c : Idx (n + 1)) (s : Tm n) : Ty (n + 1) → Ty n
+private def Ty.ren {m n : Nat} (ξ : Ren m n) : Ty m → Ty n
   | 𝑢 => 𝑢
-  | .pi ⟨x, a⟩ b => .pi ⟨x, Ty.substAt c s a⟩ (Ty.substAt c.succ (↑s) b)
-  | .el t => .el (Tm.substAt c s t)
-
-def Tm.substAt {n} (c : Idx (n + 1)) (s : Tm n) : Tm (n + 1) → Tm n
-  | .var i =>
-      if hlt : i.val < c.val then
-        .var ⟨i.val, by omega⟩
-      else if heq : i.val = c.val then
-        s
-      else
-        .var ⟨i.val - 1, by omega⟩
-  | .const name => .const name
-  | .lam ⟨x, a⟩ body => .lam ⟨x, Ty.substAt c s a⟩ (Tm.substAt c.succ (↑s) body)
-  | .app f a => .app (Tm.substAt c s f) (Tm.substAt c s a)
-  | .piHat x a b => .piHat x (Tm.substAt c s a) (Tm.substAt c.succ (↑s) b)
-  | .proj i t => .proj i (Tm.substAt c s t)
-  | .letE x ty t body => .letE x (Ty.substAt c s ty) (Tm.substAt c s t) (Tm.substAt c.succ (↑s) body)
-
+  | .pi ⟨x, a⟩ b => .pi ⟨x, a.ren ξ⟩ (b.ren ξ.up)
+  | .el t => .el (t.ren ξ)
+private def Tm.ren {m n : Nat} (ξ : Ren m n) : Tm m → Tm n
+  | .var i => .var (ξ i)
+  | .const x => .const x
+  | .lam ⟨x, a⟩ body => .lam ⟨x, a.ren ξ⟩ (body.ren ξ.up)
+  | .app f a => .app (f.ren ξ) (a.ren ξ)
+  | .piHat x a b => .piHat x (a.ren ξ) (b.ren ξ.up)
+  | .proj i t => .proj i (t.ren ξ)
+  | .letE x ty t body => .letE x (ty.ren ξ) (t.ren ξ) (body.ren ξ.up)
 end
 
-abbrev Ty.subst {n} : Tm n → Ty (n + 1) → Ty n := Ty.substAt 0
-abbrev Tm.subst {n} : Tm n → Tm (n + 1) → Tm n := Tm.substAt 0
+
+@[simp]
+private theorem Ren.up_id (n : Nat) : (Ren.id n).up = Ren.id (n + 1) := by
+  funext ⟨i, hi⟩; cases i <;> rfl
+
+@[simp]
+private theorem Ren.up_comp {l m n : Nat} (ξ : Ren l m) (ζ : Ren m n) :
+    (ξ.comp ζ).up = ξ.up.comp ζ.up := by
+  funext ⟨i, hi⟩; cases i <;> rfl
+
+mutual
+@[simp]
+private theorem Ty.ren_id {n} : ∀ A : Ty n, A.ren (Ren.id n) = A
+  | 𝑢 => rfl
+  | .pi ⟨_, _⟩ _ => by simp [Ty.ren, Ty.ren_id]
+  | .el .. => by simp [Ty.ren, Tm.ren_id]
+@[simp]
+private theorem Tm.ren_id {n} : ∀ t : Tm n, t.ren (Ren.id n) = t
+  | .var .. => rfl
+  | .const .. => rfl
+  | .lam ⟨_, _⟩ _ => by simp [Tm.ren, Ty.ren_id, Tm.ren_id]
+  | .app .. => by simp only [Tm.ren, Tm.ren_id]
+  | .piHat .. => by simp [Tm.ren, Tm.ren_id]
+  | .proj .. => by simp only [Tm.ren, Tm.ren_id]
+  | .letE .. => by simp [Tm.ren, Ty.ren_id, Tm.ren_id]
+end
+
+private theorem Ren.shift_comp {m n} (ξ : Ren m n) :
+    Ren.shift.comp ξ.up = ξ.comp Ren.shift := rfl
+
+mutual
+@[simp]
+private theorem Ty.comp_ren {l m n} (ξ : Ren l m) (ζ : Ren m n) :
+    ∀ A : Ty l, A.ren (ξ.comp ζ) = (A.ren ξ).ren ζ
+  | 𝑢 => rfl
+  | .pi ⟨_, _⟩ _ => by simp [Ty.ren, Ty.comp_ren]
+  | .el .. => by simp only [Ty.ren, Tm.comp_ren]
+@[simp]
+private theorem Tm.comp_ren {l m n} (ξ : Ren l m) (ζ : Ren m n) :
+    ∀ t : Tm l, t.ren (ξ.comp ζ) = (t.ren ξ).ren ζ
+  | .var .. => rfl
+  | .const .. => rfl
+  | .lam ⟨_, _⟩ _ => by simp [Tm.ren, Ty.comp_ren, Tm.comp_ren]
+  | .app .. => by simp only [Tm.ren, Tm.comp_ren]
+  | .piHat .. => by simp [Tm.ren, Tm.comp_ren]
+  | .proj .. => by simp only [Tm.ren, Tm.comp_ren]
+  | .letE .. => by simp [Tm.ren, Ty.comp_ren, Tm.comp_ren]
+end
+
+
+def Subst (a b : Nat) := Idx a → Tm b
+@[ext] theorem Subst.ext {a b : Nat} {σ τ : Subst a b} : (∀ i, σ i = τ i) →  σ = τ := funext
+def Subst.id (a : Nat) : Subst a a := Tm.var
+def Subst.shift {a} : Subst a (a + 1) := Subst.id (a + 1) ∘ Ren.shift
+def Subst.cons {a b} (s : Tm b) (σ : Subst a b) : Subst (a + 1) b
+  | ⟨0, _⟩ => s
+  | ⟨i + 1, h⟩ => σ ⟨i, by omega⟩
+infixr:67 " .: " => Subst.cons
+def Subst.up {m n} (σ : Subst m n) : Subst (m + 1) (n + 1) :=
+  Subst.id (n + 1) 0 .: Tm.ren Ren.shift ∘ σ
+
+@[simp]
+theorem Subst.up_id (n : Nat) : (Subst.id n).up = Subst.id (n + 1) := by
+  funext ⟨i, hi⟩; cases i <;> rfl
+
+mutual
+def Ty.subst {m n : Nat} (σ : Subst m n) : Ty m → Ty n
+  | 𝑢 => 𝑢
+  | .pi ⟨x, a⟩ b => .pi ⟨x, a.subst σ⟩ (b.subst σ.up)
+  | .el t => .el (t.subst σ)
+def Tm.subst {m n : Nat} (σ : Subst m n) : Tm m → Tm n
+  | .var i => σ i
+  | .const name => .const name
+  | .lam ⟨x, a⟩ body => .lam ⟨x, a.subst σ⟩ (body.subst σ.up)
+  | .app f a => .app (f.subst σ) (a.subst σ)
+  | .piHat x a b => .piHat x (a.subst σ) (b.subst σ.up)
+  | .proj i t => .proj i (t.subst σ)
+  | .letE x ty t body => .letE x (ty.subst σ) (t.subst σ) (body.subst σ.up)
+end
+
+@[simp]
+theorem Tm.subst_var {m n : Nat} (σ : Subst m n) (i : Idx m) : Tm.subst σ (.var i) = σ i := rfl
+
+def Subst.comp {l m n : Nat} (σ : Subst l m) (τ : Subst m n) : Subst l n := Tm.subst τ ∘ σ
+
+abbrev Ren.toSubst {m n} (ξ : Ren m n) : Subst m n := Tm.var ∘ ξ
+
+theorem Subst.subst_comp_up {m n} (ξ : Ren m n) :
+    ξ.toSubst.up = ξ.up.toSubst := by
+  funext ⟨i, hi⟩; cases i <;> rfl
+
+mutual
+theorem Ty.ren_eq_subst_var {m n} (ξ : Ren m n) :
+    ∀ A : Ty m, A.ren ξ = A.subst ξ.toSubst
+  | 𝑢 => rfl
+  | .pi ⟨_, _⟩ _ => by
+    simp only [Ty.ren, Ty.subst, Ty.ren_eq_subst_var, Subst.subst_comp_up]
+  | .el t => by simp only [Ty.ren, Ren.toSubst, Ty.subst, Tm.ren_eq_subst_var ξ t]
+theorem Tm.ren_eq_subst_var {m n} (ξ : Ren m n) :
+    ∀ t : Tm m, t.ren ξ = t.subst ξ.toSubst
+  | .var .. => rfl
+  | .const .. => rfl
+  | .lam ⟨_, _⟩ _ => by
+      simp only [Tm.ren, Tm.subst, Ty.ren_eq_subst_var, Tm.ren_eq_subst_var, Subst.subst_comp_up]
+  | .app .. => by simp only [Tm.ren, Tm.subst, Tm.ren_eq_subst_var]
+  | .piHat .. => by
+      simp only [Tm.ren, Tm.subst, Tm.ren_eq_subst_var, Subst.subst_comp_up]
+  | .proj .. => by simp only [Tm.ren, Tm.subst, Tm.ren_eq_subst_var]
+  | .letE .. => by
+      simp only [Tm.ren, Tm.subst, Ty.ren_eq_subst_var, Tm.ren_eq_subst_var, Subst.subst_comp_up]
+end
+
+section SubstitutionLemmas
+
+mutual
+@[simp]
+theorem Ty.subst_id {n} : ∀ A : Ty n, A.subst (Subst.id n) = A
+  | 𝑢 => rfl
+  | .pi ⟨_, _⟩ _ => by simp [Ty.subst, Ty.subst_id]
+  | .el .. => by simp only [Ty.subst, Tm.subst_id]
+@[simp]
+theorem Tm.subst_id {n} : ∀ t : Tm n, t.subst (Subst.id n) = t
+  | .var .. => rfl
+  | .const .. => rfl
+  | .lam ⟨_, _⟩ _ => by simp [Tm.subst, Ty.subst_id, Tm.subst_id]
+  | .app .. => by simp [Tm.subst, Tm.subst_id]
+  | .piHat .. => by simp [Tm.subst, Tm.subst_id]
+  | .proj .. => by simp only [Tm.subst, Tm.subst_id]
+  | .letE .. => by simp [Tm.subst, Ty.subst_id, Tm.subst_id]
+end
+
+@[simp]
+theorem Subst.id_comp {m n} (σ : Subst m n) : (Subst.id m).comp σ = σ := rfl
+@[simp]
+theorem Subst.comp_id {m n} (σ : Subst m n) : σ.comp (Subst.id n) = σ := by
+  funext i; apply Tm.subst_id
+
+theorem Subst.up_eq_cons_ren {m n} (σ : Subst m n) :
+    σ.up = .var 0 .: (Tm.ren Ren.shift ∘ σ) := rfl
+
+theorem Subst.cons_comp {l m n} (s : Tm m) (σ : Subst l m) (τ : Subst m n) :
+    (s .: σ).comp τ = s.subst τ .: σ.comp τ := by
+  funext ⟨i, hi⟩
+  cases i <;> rfl
+
+theorem Subst.shift_cons {n m} (s : Tm m) (σ : Subst n m) :
+    Subst.shift.comp (s .: σ) = σ := by
+  funext ⟨i, hi⟩
+  rfl
+
+private theorem Subst.comp_ren_up {l m n} (σ : Subst m n) (ξ : Ren l m) :
+    Subst.up (σ ∘ ξ) = σ.up ∘ ξ.up := by
+  funext ⟨i, hi⟩
+  cases i <;> rfl
+
+mutual
+private theorem Ty.ren_subst {l m n} (ξ : Ren l m) (σ : Subst m n) :
+    (A : Ty l) → (A.ren ξ).subst σ = A.subst (σ ∘ ξ)
+  | 𝑢 => rfl
+  | .pi ⟨_, _⟩ _ => by simp only [Ty.ren, Ty.subst, Ty.ren_subst, Subst.comp_ren_up]
+  | .el .. => by simp only [Ty.ren, Ty.subst, Tm.ren_subst]
+private theorem Tm.ren_subst {l m n} (ξ : Ren l m) (σ : Subst m n) :
+    ∀ t : Tm l, (t.ren ξ).subst σ = t.subst (σ ∘ ξ)
+  | .var .. => rfl
+  | .const .. => rfl
+  | .lam ⟨_, _⟩ _ => by simp only [Tm.ren, Tm.subst, Ty.ren_subst, Tm.ren_subst, Subst.comp_ren_up]
+  | .app .. => by simp only [Tm.ren, Tm.subst, Tm.ren_subst]
+  | .piHat .. => by simp only [Tm.ren, Tm.subst, Tm.ren_subst, Subst.comp_ren_up]
+  | .proj .. => by simp only [Tm.ren, Tm.subst, Tm.ren_subst]
+  | .letE .. => by simp only [Tm.ren, Tm.subst, Ty.ren_subst, Tm.ren_subst, Subst.comp_ren_up]
+end
+
+private theorem Subst.ren_comp_up {l m n} (σ : Subst l m) (ξ : Ren m n) :
+    Subst.up (Tm.ren ξ ∘ σ) = Tm.ren ξ.up ∘ σ.up := by
+  funext ⟨i, hi⟩
+  cases i with
+  | zero => rfl
+  | succ _ => simp only [up, cons, Function.comp_apply, ← Tm.comp_ren, Ren.shift_comp]
+
+mutual
+private theorem Ty.subst_ren {l m n} (σ : Subst l m) (ξ : Ren m n) :
+    ∀ A : Ty l, (A.subst σ).ren ξ = A.subst (Tm.ren ξ ∘ σ)
+  | 𝑢 => rfl
+  | .pi ⟨_, _⟩ _ => by simp only [Ty.subst, Ty.ren, Ty.subst_ren, Subst.ren_comp_up]
+  | .el .. => by simp only [Ty.subst, Ty.ren, Tm.subst_ren]
+private theorem Tm.subst_ren {l m n} (σ : Subst l m) (ξ : Ren m n) :
+    ∀ t : Tm l, (t.subst σ).ren ξ = t.subst (Tm.ren ξ ∘ σ)
+  | .var .. => rfl
+  | .const .. => rfl
+  | .lam ⟨_, _⟩ _ => by simp only [Tm.subst, Tm.ren, Ty.subst_ren, Tm.subst_ren, Subst.ren_comp_up]
+  | .app .. => by simp only [Tm.subst, Tm.ren, Tm.subst_ren]
+  | .piHat .. => by simp only [Tm.subst, Tm.ren, Tm.subst_ren, Subst.ren_comp_up]
+  | .proj .. => by simp only [Tm.subst, Tm.ren, Tm.subst_ren]
+  | .letE .. => by simp only [Tm.subst, Tm.ren, Ty.subst_ren, Tm.subst_ren, Subst.ren_comp_up]
+end
+
+theorem Subst.shift_up_comm {m n} (σ : Subst m n) :
+    shift.comp σ.up = σ.comp shift := by
+  funext ⟨i, hi⟩
+  simp [shift]
+  apply Tm.ren_eq_subst_var
+
+
+@[simp]
+theorem Subst.up_comp {l m n} (σ : Subst l m) (τ : Subst m n) :
+    (σ.comp τ).up = σ.up.comp τ.up := by
+  funext ⟨i, hi⟩
+  cases i with
+  | zero => rfl
+  | succ i =>
+    simp [Subst.up, Subst.cons, Subst.comp, Tm.subst_ren, Tm.ren_subst]
+    rfl
+
+mutual
+@[simp]
+theorem Ty.comp_subst {l m n} (σ : Subst l m) (τ : Subst m n) :
+    ∀ A : Ty l, (A.subst σ).subst τ = A.subst (σ.comp τ)
+  | 𝑢 => rfl
+  | .pi ⟨x, a⟩ b => by simp only [Ty.subst, Ty.comp_subst, Subst.up_comp]
+  | .el t => by simp only [Ty.subst, Tm.comp_subst]
+
+@[simp]
+theorem Tm.comp_subst {l m n} (σ : Subst l m) (τ : Subst m n) :
+    ∀ t : Tm l, (t.subst σ).subst τ = t.subst (σ.comp τ)
+  | .var .. => rfl
+  | .const .. => rfl
+  | .lam ⟨_, _⟩ _ => by simp only [Tm.subst, Ty.comp_subst, Tm.comp_subst, Subst.up_comp]
+  | .app .. => by simp only [Tm.subst, Tm.comp_subst]
+  | .piHat .. => by simp only [Tm.subst, Tm.comp_subst, Subst.up_comp]
+  | .proj .. => by simp only [Tm.subst, Tm.comp_subst]
+  | .letE .. => by simp only [Tm.subst, Ty.comp_subst, Tm.comp_subst, Subst.up_comp]
+end
+
+theorem Subst.comp_assoc {k l m n} (σ : Subst k l) (τ : Subst l m) (ρ : Subst m n) :
+    (σ.comp τ).comp ρ = σ.comp (τ.comp ρ) := by
+  funext i
+  simp only [Subst.comp, Function.comp_apply]
+  exact Tm.comp_subst τ ρ (σ i)
+
+end SubstitutionLemmas
+
+-- Substitutions form a category
+
+-- open CategoryTheory
+
+-- structure Subst.Obj where
+--   n : Nat
+
+-- instance : Coe Subst.Obj Nat where
+--   coe := Subst.Obj.n
+
+-- instance : Category Subst.Obj where
+--   id n := Subst.id n
+--   Hom m n := Subst m n
+--   comp σ τ := Subst.comp σ τ
+--   id_comp σ := Subst.id_comp σ
+--   comp_id σ := Subst.comp_id σ
+--   assoc σ τ ρ := Subst.comp_assoc σ τ ρ
+
+-- def Subst.upFunctor : Subst.Obj ⥤ Subst.Obj where
+--   obj n := ⟨n + 1⟩
+--   map := Subst.up
+--   map_id n := Subst.up_id n
+--   map_comp := Subst.up_comp
+
+theorem Ren.toSubst_up {m n} (ξ : Ren m n) :
+    Subst.up (Ren.toSubst ξ) = Ren.toSubst (Ren.up ξ) :=
+  Subst.subst_comp_up ξ
+
+def Subst.beta {n : Nat} (s : Tm n) : Subst (n + 1) n := s .: Subst.id n
+
+@[simp]
+theorem Subst.shift_beta {n} (s : Tm n) :
+    shift.comp (beta s) = id n :=
+  rfl
+
+@[simp]
+theorem Ty.shift_beta {n} (A : Ty n) (s : Tm n) :
+    (A.subst Subst.shift).subst (Subst.beta s) = A := by
+  rw [Ty.comp_subst, Subst.shift_beta, Ty.subst_id]
+
+@[simp]
+theorem Tm.shift_beta {n} (t : Tm n) (s : Tm n) :
+    (t.subst Subst.shift).subst (Subst.beta s) = t := by
+  rw [Tm.comp_subst, Subst.shift_beta, Tm.subst_id]
+
+@[simp]
+theorem Tm.var_zero_beta {n} (s : Tm n) : (Tm.var 0).subst (Subst.beta s) = s := rfl
+
+@[simp]
+theorem Tm.var_succ_beta {n} (i : Idx n) (s : Tm n) :
+    (Tm.var i.succ).subst (Subst.beta s) = Tm.var i := rfl
+
+theorem Subst.beta_up_zero {n} (s : Tm n) : (beta s).up 0 = Tm.var 0 := rfl
+
+theorem Subst.beta_up_one {n} (s : Tm n) : (beta s).up 1 = s.subst shift := by
+  simp only [up, beta, cons, Function.comp_apply]
+  exact Tm.ren_eq_subst_var Ren.shift s
+
+theorem Subst.beta_up_succ_succ {n} (s : Tm n) (i : Idx n) :
+    (beta s).up i.succ.succ = Tm.var i.succ := rfl
+
+theorem Subst.beta_comp_shift {n} (s : Tm n) : beta s ∘ Ren.shift = id n := by
+  funext i; rfl
+
+theorem Subst.cons_id_comp_shift {n} (s : Tm n) :
+    (s .: Tm.var) ∘ Ren.shift = Tm.var := by
+  funext i; rfl
+
+theorem Subst.beta_comp_up {m n} (a : Tm m) (σ : Subst m n) :
+    (Subst.beta a).comp σ = σ.up.comp (Subst.beta (a.subst σ)) := by
+  ext ⟨i, hi⟩
+  cases i with
+  | zero => rfl
+  | succ j =>
+    simp only [comp, beta, cons, id, up, Function.comp_apply, Tm.ren_subst, cons_id_comp_shift]
+    exact (Tm.subst_id (σ ⟨j, by omega⟩)).symm
+
+theorem Ty.beta_comp_up {m n} (A : Ty (m + 1)) (a : Tm m) (σ : Subst m n) :
+    (A.subst (Subst.beta a)).subst σ = (A.subst σ.up).subst (Subst.beta (a.subst σ)) := by
+  rw [Ty.comp_subst, Ty.comp_subst, Subst.beta_comp_up]
+
+theorem Tm.beta_comp_up {m n} (t : Tm (m + 1)) (a : Tm m) (σ : Subst m n) :
+    (t.subst (Subst.beta a)).subst σ = (t.subst σ.up).subst (Subst.beta (a.subst σ)) := by
+  rw [comp_subst, comp_subst, Subst.beta_comp_up]
+
+theorem Subst.beta_comp_beta {n} (a : Tm (n + 1)) (b : Tm n) :
+    (beta a).comp (beta b) = (a.subst (beta b)) .: b .: id n := by
+  funext ⟨i, hi⟩
+  cases i <;> rfl
+
+theorem Subst.beta_up_comp_beta {n} (a : Tm n) (b : Tm n) :
+    (beta a).up.comp (beta b) = b .: a .: id n := by
+  ext ⟨i, hi⟩
+  cases i with
+  | zero => rfl
+  | succ j =>
+    cases j with
+    | zero =>
+      simp only [Subst.comp, Function.comp_apply, Subst.up, Subst.cons]
+      rw [Tm.ren_eq_subst_var]
+      exact Tm.shift_beta a b
+    | succ k => rfl
+
+theorem Subst.beta_up_comp_beta_up {n} (a : Tm (n + 1)) (b : Tm n) :
+    (beta a).up.comp (beta b).up = ((beta a).comp (beta b)).up := by
+  rw [← Subst.up_comp]
+
+theorem Subst.beta_up_comp_up {m n} (a : Tm m) (σ : Subst m n) :
+    (beta a).up.comp σ.up = σ.up.up.comp (beta (a.subst σ)).up := by
+  rw [← up_comp, ← up_comp, beta_comp_up]
+
+theorem Ty.beta_comp_beta {n} (A : Ty (n + 2)) (a : Tm (n + 1)) (b : Tm n) :
+    (A.subst (Subst.beta a)).subst (Subst.beta b) =
+    A.subst ((Subst.beta a).comp (Subst.beta b)) := by
+  rw [Ty.comp_subst]
+
+theorem Tm.beta_comp_beta {n} (t : Tm (n + 2)) (a : Tm (n + 1)) (b : Tm n) :
+    (t.subst (Subst.beta a)).subst (Subst.beta b) =
+    t.subst ((Subst.beta a).comp (Subst.beta b)) := by
+  rw [Tm.comp_subst]
+
+theorem Subst.cons_shift_comp {m n} (s : Tm n) (σ : Subst m n) :
+    shift.comp (s .: σ) = σ := shift_cons s σ
+
+prefix:50 "↑" => Ty.subst Subst.shift
+prefix:50 "↑" => Tm.subst Subst.shift
+
+abbrev Tm.weaken {n} : Tm n → Tm (n + 1) := Tm.subst Subst.shift
+abbrev Ty.weaken {n} : Ty n → Ty (n + 1) := Ty.subst Subst.shift
+
+abbrev Tm.subst1 {n} : Tm n → Tm (n + 1) → Tm n := Tm.subst ∘ Subst.beta
+abbrev Ty.subst1 {n} : Tm n → Ty (n + 1) → Ty n := Ty.subst ∘ Subst.beta
 
 instance {n} : GetElem (Tm (n + 1)) (Tm n) (Tm n) fun _ _ => True where
-  getElem t i _ := Tm.subst i t
+  getElem t i _ := Tm.subst1 i t
 
 instance {n} : GetElem (Ty (n + 1)) (Tm n) (Ty n) fun _ _ => True where
-  getElem t i _ := Ty.subst i t
+  getElem t i _ := Ty.subst1 i t
 
-private theorem Idx.shift_substAt_comm {n}
-    (a : Tm n)
-    (c : Idx (n + 1))
-    (k : Nat) :
-    (i : Idx (n + 1)) →
-    Tm.substAt c.castSucc (a.shiftAfter (k + c.val) 1) (Tm.var (Idx.shiftAfter (k + c.val + 1) 1 i)) =
-    (Tm.substAt c a (Tm.var i)).shiftAfter (k + c.val) 1
-  | ⟨j, hj⟩ => by
-      unfold Tm.substAt Idx.shiftAfter Fin.castSucc
-      by_cases hjc : j < c.val
-      · have h1 : ¬ k + c.val + 1 ≤ j := by omega
-        have h2 : ¬ k + c.val ≤ j := by omega
-        simp [h1, hjc, h2, Tm.shiftAfter, Idx.shiftAfter]
-      by_cases hjc' : j = c.val
-      · have : ¬ k + c.val + 1 ≤ c.val := by omega
-        simp [hjc', this]
-      · have hgt : c.val < j := by omega
-        have hcc : (Fin.castAdd 1 c).val = c.val := rfl
-        by_cases hk : k + c.val + 1 ≤ j
-        all_goals simp only [hk, hcc, hjc, hjc', ↓reduceIte, dite_false]
-        case pos =>
-          have h₁ : ¬ j + 1 < c.val := by omega
-          have h₂ : j + 1 ≠ c.val := by omega
-          have h₃ : k + c.val ≤ j - 1 := by omega
-          have hj₁ : j + 1 - 1 = j := by omega
-          have hj₂ : j - 1 + 1 = j := by omega
-          simp [h₁, h₂, h₃, hj₁, hj₂, Tm.shiftAfter, Idx.shiftAfter]
-        case neg =>
-          have h : ¬ k + c.val ≤ j - 1 := by omega
-          simp [h, Tm.shiftAfter, Idx.shiftAfter]
+def Ren.upN {m n : Nat} : ∀ k, Ren m n → Ren (m + k) (n + k)
+  | 0 => _root_.id
+  | k + 1 => up ∘ upN k
 
-private theorem ha {n} (a : Tm n) (k : Nat) (c : Idx (n + 1)) :
-    (a.shift 1).shiftAfter (k + c.val + 1) 1 = (a.shiftAfter (k + c.val) 1).shift 1 :=
-  Tm.shift_shift_comm_gen 0 (k + c.val) a
+def Subst.upN {m n : Nat} : ∀ k, Subst m n → Subst (m + k) (n + k)
+  | 0 => _root_.id
+  | k + 1 => up ∘ upN k
 
-private theorem add_succ_val {n} (c : Idx (n + 1)) (k : Nat) :
-    k + c.val + 1 = k + c.succ.val := rfl
+@[simp] theorem Ren.upN_zero {m n : Nat} (ξ : Ren m n) : Ren.upN 0 ξ = ξ := rfl
+@[simp] theorem Ren.upN_succ {m n : Nat} (k : Nat) (ξ : Ren m n) : Ren.upN (k + 1) ξ = (Ren.upN k ξ).up := rfl
+@[simp] theorem Subst.upN_zero {m n : Nat} (σ : Subst m n) : Subst.upN 0 σ = σ := rfl
+@[simp] theorem Subst.upN_succ {m n : Nat} (k : Nat) (σ : Subst m n) : Subst.upN (k + 1) σ = (Subst.upN k σ).up := rfl
 
-mutual
+@[simp]
+theorem Ren.id_upN {n : Nat} : ∀ k, (Ren.id n).upN k = Ren.id (n + k)
+  | 0 => rfl
+  | k + 1 => by simp [Ren.id_upN]; rfl
 
-theorem Ty.shift_substAt_comm {n}
-    (c : Idx (n + 1))
-    (k : Nat)
-    (a : Tm n) :
-    (B : Ty (n + 1)) →
-    Ty.substAt c.castSucc (a.shiftAfter (k + c.val) 1) (B.shiftAfter (k + c.val + 1) 1) =
-    (Ty.substAt c a B).shiftAfter (k + c.val) 1
-  | 𝑢 => by simp only [Ty.shiftAfter, Ty.substAt]
-  | .pi ⟨x, A⟩ B => by
-      simp only [Ty.shiftAfter, Ty.substAt]
-      congr 2
-      · exact Ty.shift_substAt_comm c k a A
-      · rw [Fin.succ_castSucc, ← ha, add_succ_val]
-        exact Ty.shift_substAt_comm c.succ k (↑a) B
-  | .el .. => by
-      simp only [Ty.shiftAfter, Ty.substAt]
+@[simp]
+theorem Subst.id_upN {n : Nat} : ∀ k, (Subst.id n).upN k = Subst.id (n + k)
+  | 0 => rfl
+  | k + 1 => by simp [Subst.id_upN]; rfl
+
+theorem Ren.comp_upN {l m n : Nat} (ξ : Ren l m) (ζ : Ren m n) :
+    ∀ k, (ξ.comp ζ).upN k = (ξ.upN k).comp (ζ.upN k)
+  | 0 => rfl
+  | k + 1 => by simp [Ren.comp_upN, Ren.up_comp]
+
+theorem Subst.comp_upN {l m n : Nat} (σ : Subst l m) (τ : Subst m n) :
+    ∀ k, (σ.comp τ).upN k = (σ.upN k).comp (τ.upN k)
+  | 0 => rfl
+  | k + 1 => by simp [Subst.comp_upN]
+
+theorem Subst.shift_upN_beta {n : Nat} (s : Tm n) :
+    ∀ k, (Subst.shift.upN k).comp ((Subst.beta s).upN k) = (Subst.id n).upN k
+  | 0 => Subst.shift_beta s
+  | k + 1 => by
+      simp only [Subst.upN_succ, ← Subst.up_comp]
       congr 1
-      · apply Tm.shift_substAt_comm
+      exact Subst.shift_upN_beta s k
 
-theorem Tm.shift_substAt_comm {n}
-    (c : Idx (n + 1))
-    (k : Nat)
-    (a : Tm n) :
-    (b : Tm (n + 1)) →
-    Tm.substAt c.castSucc (a.shiftAfter (k + c.val) 1) (b.shiftAfter (k + c.val + 1) 1) =
-    (Tm.substAt c a b).shiftAfter (k + c.val) 1
-  | .var .. => by apply Idx.shift_substAt_comm
-  | .const .. => by simp only [Tm.shiftAfter, Tm.substAt]
-  | .lam ⟨x, A⟩ body => by
-      simp only [Tm.shiftAfter, Tm.substAt]
-      congr 2
-      · exact Ty.shift_substAt_comm c k a A
-      · rw [Fin.succ_castSucc, ← ha, add_succ_val]
-        exact Tm.shift_substAt_comm c.succ k (↑a) body
-  | .app .. => by
-      simp only [Tm.shiftAfter, Tm.substAt]
-      congr 1
-      · apply Tm.shift_substAt_comm
-      · apply Tm.shift_substAt_comm
-  | .piHat .. => by
-      simp only [Tm.shiftAfter, Tm.substAt]
-      congr 1
-      · apply Tm.shift_substAt_comm
-      · rw [← ha, Fin.succ_castSucc, add_succ_val]
-        apply Tm.shift_substAt_comm
-  | .proj .. => by
-      simp only [Tm.shiftAfter, Tm.substAt]
-      congr 1
-      · apply Tm.shift_substAt_comm
-  | .letE .. => by
-      simp only [Tm.shiftAfter, Tm.substAt]
-      congr 1
-      · apply Ty.shift_substAt_comm
-      · apply Tm.shift_substAt_comm
-      · rw [← ha, Fin.succ_castSucc, add_succ_val]
-        apply Tm.shift_substAt_comm
+private def Ren.shiftN {a} : (s : Nat) → Ren a (a + s)
+  | 0 => Ren.id a
+  | s + 1 => Ren.comp (Ren.shiftN s) Ren.shift
 
-end
+private def Idx.shiftAfter (n k s : Nat) : Ren n (n + s) :=
+  match k with
+  | 0 => Ren.shiftN s
+  | k + 1 => match n with
+    | 0 => Ren.shiftN s
+    | n + 1 => Nat.add_right_comm n 1 s ▸ Ren.up (Idx.shiftAfter n k s)
 
-theorem Ty.shift_subst_comm {n} :
-    ∀ k (a : Tm n) (B : Ty (n + 1)),
-    (B.shiftAfter (k + 1) 1)[a.shiftAfter k 1] = B[a].shiftAfter k 1 :=
-  Ty.shift_substAt_comm 0
+def Ty.shiftAfter {n : Nat} (k s : Nat) : Ty n → Ty (n + s) :=
+  Ty.ren (Idx.shiftAfter n k s)
 
-theorem Tm.shift_subst_comm {n} :
-    ∀ k (a : Tm n) (b : Tm (n + 1)),
-    (b.shiftAfter (k + 1) 1)[a.shiftAfter k 1] = b[a].shiftAfter k 1 :=
-  Tm.shift_substAt_comm 0
+def Tm.shiftAfter {n : Nat} (k s : Nat) : Tm n → Tm (n + s) :=
+  Tm.ren (Idx.shiftAfter n k s)
+
+abbrev Ty.shift {n : Nat} : ∀ s, Ty n → Ty (n + s) := Ty.shiftAfter 0
+abbrev Tm.shift {n : Nat} : ∀ s, Tm n → Tm (n + s) := Tm.shiftAfter 0
+
+private unsafe def Tm.wkClosed_impl {n : Nat} : Tm 0 → Tm n := unsafeCast
+private unsafe def Ty.wkClosed_impl {n : Nat} : Ty 0 → Ty n := unsafeCast
+@[implemented_by Tm.wkClosed_impl]
+def Tm.wkClosed {n : Nat} (t : Tm 0) : Tm n := Nat.zero_add n ▸ t.shift n
+@[implemented_by Ty.wkClosed_impl]
+def Ty.wkClosed {n : Nat} (t : Ty 0) : Ty n := Nat.zero_add n ▸ t.shift n
+
+@[simp]
+private theorem Ren.shiftN_zero {a} : Ren.shiftN 0 = Ren.id a := rfl
+
+@[simp]
+private theorem Ren.shiftN_one {a} : Ren.shiftN 1 = (Ren.shift : Ren a (a + 1)) := by
+  simp [Ren.shiftN, Ren.id_comp]
+
+private theorem Ren.shiftN_succ {a} (s : Nat) :
+    (Ren.shiftN (s + 1) : Ren a (a + s + 1)) = Ren.comp (Ren.shiftN s) Ren.shift := rfl
+
+def Subst.shiftN {n} : (s : Nat) → Subst n (n + s)
+  | 0 => Subst.id n
+  | s + 1 => Subst.comp (Subst.shiftN s) Subst.shift
+
+@[simp]
+theorem Subst.shiftN_zero {n} : Subst.shiftN 0 = Subst.id n := rfl
+
+@[simp]
+theorem Subst.shiftN_one {n} : Subst.shiftN 1 = (Subst.shift : Subst n (n + 1)) := by
+  simp only [Subst.shiftN, Subst.id_comp]
+
+theorem Subst.shiftN_succ {n} (s : Nat) :
+    (Subst.shiftN (s + 1) : Subst n (n + s + 1)) = Subst.comp (Subst.shiftN s) Subst.shift := rfl
 
 end Qdt
