qdt/Qdt/MLTT.lean
@@ -1,10 +1,9 @@
 import Qdt.MLTT.AlphaEq
 import Qdt.MLTT.Bidirectional
 import Qdt.MLTT.Context
-import Qdt.MLTT.Judgements
+import Qdt.MLTT.Declarative
+import Qdt.MLTT.Global
 import Qdt.MLTT.Plausible
-import Qdt.MLTT.Shift
 import Qdt.MLTT.Substitution.Basic
-import Qdt.MLTT.Substitution.Theorem
 import Qdt.MLTT.Syntax
 import Qdt.MLTT.Weakening
